Some cleanup, invariant
Some minor cleanup work was done to perhaps present this in the thesis, but I decided this will not happen in the draft (yet).

Will make a final decision after an upcoming meeting.

TangleLearning_Solve.thy
@@ -2,56 +2,68 @@ theory TangleLearning_Solve
   imports Main ParityGames TangleAttractors TangleLearning_Search
 begin
 
+type_synonym 'a solve_state =
+  "'a set \<times> 'a set \<times> 'a strat \<times> 'a strat \<times> 'a set \<times> 'a set set"
+
 context paritygame begin
 
-type_synonym 'a solve_state = "'a set \<times> 'a set \<times> 'a strat \<times> 'a strat \<times> 'a set \<times> 'a set set"
-definition solve_state_W\<^sub>0 :: "'a solve_state \<Rightarrow> 'a set" where
-  "solve_state_W\<^sub>0 \<equiv> \<lambda>(W\<^sub>0,W\<^sub>1,\<sigma>\<^sub>0,\<sigma>\<^sub>1,R,T). W\<^sub>0"
+abbreviation (input) filter_T :: "'v set set \<Rightarrow>  player \<Rightarrow> 'v set set" where
+  "filter_T T \<alpha> \<equiv> {t. t\<in>T \<and> tangle EVEN t}"
 
-definition solve_state_W\<^sub>1 :: "'a solve_state \<Rightarrow> 'a set" where
-  "solve_state_W\<^sub>1 \<equiv> \<lambda>(W\<^sub>0,W\<^sub>1,\<sigma>\<^sub>0,\<sigma>\<^sub>1,R,T). W\<^sub>1"
-
-definition solve_state_\<sigma>\<^sub>0 :: "'a solve_state \<Rightarrow> 'a strat" where
-  "solve_state_\<sigma>\<^sub>0 \<equiv> \<lambda>(W\<^sub>0,W\<^sub>1,\<sigma>\<^sub>0,\<sigma>\<^sub>1,R,T). \<sigma>\<^sub>0"
-
-definition solve_state_\<sigma>\<^sub>1 :: "'a solve_state \<Rightarrow> 'a strat" where
-  "solve_state_\<sigma>\<^sub>1 \<equiv> \<lambda>(W\<^sub>0,W\<^sub>1,\<sigma>\<^sub>0,\<sigma>\<^sub>1,R,T). \<sigma>\<^sub>1"
-
-definition solve_state_R :: "'a solve_state \<Rightarrow> 'a set" where
-  "solve_state_R \<equiv> \<lambda>(W\<^sub>0,W\<^sub>1,\<sigma>\<^sub>0,\<sigma>\<^sub>1,R,T). R"
-
-definition solve_state_T :: "'a solve_state \<Rightarrow> 'a set set" where
-  "solve_state_T \<equiv> \<lambda>(W\<^sub>0,W\<^sub>1,\<sigma>\<^sub>0,\<sigma>\<^sub>1,R,T). T"
+abbreviation (input) filter_D :: "('v set \<times> 'v strat) set \<Rightarrow> player \<Rightarrow> 'v set set" where
+  "filter_D D \<alpha> \<equiv> {U | U \<sigma>. (U,\<sigma>)\<in>D \<and> strategy_of_player \<alpha> \<sigma>}"
 
 inductive solve_step :: "'v solve_state \<Rightarrow> 'v solve_state \<Rightarrow> bool" where
-  step: "\<lbrakk>R\<noteq>{}; R \<subseteq> V; paritygame (Restr E R) (V\<inter>R) (V\<^sub>0\<inter>R);
-          search T R Y;
-          T' = T \<union> {U | U \<sigma> \<alpha>. U \<in> Y \<and> tangle_strat \<alpha> U \<sigma> \<and> (E `` (U\<inter>V_opponent \<alpha>)) - U \<noteq> {}};
-          T\<^sub>0' = {t. t\<in>T' \<and> tangle EVEN t}; T\<^sub>1' = {t. t \<in> T' \<and> tangle ODD t};
-          D = {(U,\<sigma>) | U \<sigma> \<alpha>. U \<in> Y \<and> tangle_strat \<alpha> U \<sigma> \<and> (E `` (U\<inter>V_opponent \<alpha>)) \<subseteq> U};
-          D\<^sub>0 = {U | U \<sigma>. (U,\<sigma>) \<in> D \<and> strategy_of_player EVEN \<sigma>};
-          D\<^sub>1 = {U | U \<sigma>. (U,\<sigma>) \<in> D \<and> strategy_of_player ODD \<sigma>};
-          tangle_attractor EVEN T\<^sub>0' (\<Union>D\<^sub>0) W\<^sub>0'' \<sigma>\<^sub>0'';
-          tangle_attractor ODD T\<^sub>1' (\<Union>D\<^sub>1) W\<^sub>1'' \<sigma>\<^sub>1'';
-          W\<^sub>0' = (if D\<noteq>{} then W\<^sub>0 \<union> W\<^sub>0'' else W\<^sub>0);
-          \<sigma>\<^sub>0' = (if D\<noteq>{} then \<sigma>\<^sub>0 ++ \<sigma>\<^sub>0'' else \<sigma>\<^sub>0);
-          W\<^sub>1' = (if D\<noteq>{} then W\<^sub>1 \<union> W\<^sub>1'' else W\<^sub>1);
-          \<sigma>\<^sub>1' = (if D\<noteq>{} then \<sigma>\<^sub>1 ++ \<sigma>\<^sub>1'' else \<sigma>\<^sub>1);
-          R' = (if D\<noteq>{} then R - (W\<^sub>0'\<union>W\<^sub>1') else R)\<rbrakk>
-            \<Longrightarrow> solve_step (W\<^sub>0,W\<^sub>1,\<sigma>\<^sub>0,\<sigma>\<^sub>1,R,T) (W\<^sub>0',W\<^sub>1',\<sigma>\<^sub>0',\<sigma>\<^sub>1',R',T')"
+  step:
+  "\<lbrakk>R\<noteq>{};
+    search T R Y;
+    T' = T \<union> {U | U \<sigma> \<alpha>. U \<in> Y \<and> tangle_strat \<alpha> U \<sigma> \<and> (E `` (U\<inter>V_opponent \<alpha>)) - U \<noteq> {}};
+    D = {(U,\<sigma>) | U \<sigma> \<alpha>. U \<in> Y \<and> tangle_strat \<alpha> U \<sigma> \<and> (E `` (U\<inter>V_opponent \<alpha>)) \<subseteq> U};
+    tangle_attractor EVEN (filter_T T EVEN) (\<Union>(filter_D D EVEN)) W\<^sub>0'' \<sigma>\<^sub>0'';
+    tangle_attractor ODD (filter_T T ODD) (\<Union>(filter_D D ODD)) W\<^sub>1'' \<sigma>\<^sub>1'';
+    W\<^sub>0' = (if D\<noteq>{} then W\<^sub>0 \<union> W\<^sub>0'' else W\<^sub>0);
+    \<sigma>\<^sub>0' = (if D\<noteq>{} then \<sigma>\<^sub>0 ++ \<sigma>\<^sub>0'' else \<sigma>\<^sub>0);
+    W\<^sub>1' = (if D\<noteq>{} then W\<^sub>1 \<union> W\<^sub>1'' else W\<^sub>1);
+    \<sigma>\<^sub>1' = (if D\<noteq>{} then \<sigma>\<^sub>1 ++ \<sigma>\<^sub>1'' else \<sigma>\<^sub>1);
+    R' = (if D\<noteq>{} then R - (W\<^sub>0'\<union>W\<^sub>1') else R)\<rbrakk>
+      \<Longrightarrow> solve_step (W\<^sub>0,W\<^sub>1,\<sigma>\<^sub>0,\<sigma>\<^sub>1,R,T) (W\<^sub>0',W\<^sub>1',\<sigma>\<^sub>0',\<sigma>\<^sub>1',R',T')"
 
-lemma solve_step_R_notempty: "solve_step S S' \<Longrightarrow> solve_state_R S \<noteq> {}"
-  unfolding solve_state_R_def
-  apply (induction rule: solve_step.induct)
-  by fast
+lemmas solve_step_induct[consumes 1, case_names step] =
+  solve_step.induct[
+  of "(W\<^sub>0,W\<^sub>1,\<sigma>\<^sub>0,\<sigma>\<^sub>1,R,T)" "(W\<^sub>0',W\<^sub>1',\<sigma>\<^sub>0',\<sigma>\<^sub>1',R',T')"
+    for W\<^sub>0 W\<^sub>1 \<sigma>\<^sub>0 \<sigma>\<^sub>1 R T W\<^sub>0' W\<^sub>1' \<sigma>\<^sub>0' \<sigma>\<^sub>1' R' T',
+  where P="\<lambda>(a,b,c,d,e,f) (g,h,i,j,k,l). P a b c d e f g h i j k l"
+    for P,
+  unfolded split]
+
+definition solve_step_I :: "'v solve_state \<Rightarrow> bool" where
+  "solve_step_I \<equiv> \<lambda>(W\<^sub>0,W\<^sub>1,\<sigma>\<^sub>0,\<sigma>\<^sub>1,R,T).
+    valid_subgame R \<and> winning_region EVEN W\<^sub>0 \<and> winning_region ODD W\<^sub>1 \<and> finite T \<and>
+    (\<forall>t\<in>T. tangle EVEN t \<or> tangle ODD t) \<and> (\<forall>t\<in>T. \<forall>\<alpha>. tangle \<alpha> t \<longrightarrow> E `` (t\<inter>V_opponent \<alpha>)-t\<noteq>{})"
+
+lemma valid_subgame_Un:
+  "\<lbrakk>valid_subgame R; valid_subgame R'\<rbrakk> \<Longrightarrow> valid_subgame (R\<union>R')"
+  apply clarsimp
+  apply (unfold_locales; clarsimp)
+  subgoal by blast
+  subgoal for v using succ[of v] sorry
+  subgoal by blast
+  done
+
+lemma "\<lbrakk>solve_step (W\<^sub>0,W\<^sub>1,\<sigma>\<^sub>0,\<sigma>\<^sub>1,R,T) (W\<^sub>0',W\<^sub>1',\<sigma>\<^sub>0',\<sigma>\<^sub>1',R',T'); valid_subgame R\<rbrakk>
+        \<Longrightarrow> R' \<subseteq> R"
+  by (induction rule: solve_step_induct) auto
+
+lemma solve_step_R_notempty:
+  "solve_step (W\<^sub>0,W\<^sub>1,\<sigma>\<^sub>0,\<sigma>\<^sub>1,R,T) (W\<^sub>0',W\<^sub>1',\<sigma>\<^sub>0',\<sigma>\<^sub>1',R',T') \<Longrightarrow> R \<noteq> {}"
+  by (induction rule: solve_step_induct) blast
 
 definition solve :: "'v set \<Rightarrow> 'v set \<Rightarrow> 'v strat \<Rightarrow> 'v strat \<Rightarrow> bool" where
   "solve W\<^sub>0 W\<^sub>1 \<sigma>\<^sub>0 \<sigma>\<^sub>1 \<equiv> \<exists>T. solve_step\<^sup>*\<^sup>* ({},{},Map.empty,Map.empty,V,{}) (W\<^sub>0,W\<^sub>1,\<sigma>\<^sub>0,\<sigma>\<^sub>1,{},T)"
 
 lemma solve_terminates_on_empty_R: "\<not>Domainp solve_step (W\<^sub>0,W\<^sub>1,\<sigma>\<^sub>0,\<sigma>\<^sub>1,{},T)"
-  using solve_step_R_notempty
-  unfolding solve_state_R_def
-  by fast
+  using solve_step_R_notempty by fast
+
 
 lemma tanglelearning_terminates:
   "\<exists>W\<^sub>0 W\<^sub>1 \<sigma>\<^sub>0 \<sigma>\<^sub>1. solve W\<^sub>0 W\<^sub>1 \<sigma>\<^sub>0 \<sigma>\<^sub>1"
